\documentclass[12pt]{article}
\usepackage{amsmath,amssymb,amsthm}
\usepackage{graphicx}
\usepackage{fullpage}
\usepackage[innercaption]{sidecap}
\newcommand{\estart}
{
\renewcommand{\labelenumi}{(\alph{enumi})}
\vspace{-0.5\baselineskip}
\begin{enumerate}
}

\newcommand{\eend}
{
\end{enumerate}
\renewcommand{\labelenumi}{(\arabic{enumi})}
}

\usepackage{rotating}


\usepackage[absolute]{textpos}
\setlength{\TPHorizModule}{1mm}
\setlength{\TPVertModule}{1mm}

\begin{document}

\pagestyle{empty}

\section*{Summary: Linear Least Squares (Chapter 8)}

\begin{textblock}{170}(10,260)
\noindent \textsf{{\small Intro Scientific Computing and Data Analysis, M. H. Holmes, 2nd ed (version: \today)}}
\end{textblock}

\bigskip\bigskip\noindent
\textbf{Basic: $y=v_1+v_2x$}

\bigskip\noindent
Error Function:
\[
E(v_1,v_2) = \sum_{i=1}^n (v_1+v_2x_i - y_i)^2
\tag{8.9}
\]

Solution:
\[
\begin{pmatrix}
v_1  \medskip\\
v_2
\end{pmatrix}
=
\frac{1}{n\sum x_i^2 - \big (\sum x_i \big)^2} \!
\begin{pmatrix}
\,\, \sum x_i^2 & -\sum x_i  \\[0.4em]
-\sum x_i & \quad n 
\end{pmatrix}
\!\!\!
\begin{pmatrix}
\sum  y_i  \medskip\\
\sum  x_iy_i 
\end{pmatrix}
\tag{8.11}
\]

\bigskip\bigskip\noindent
Error Function:
\[
E(v_1,v_2) = \sum_{i=1}^n \! \left ( \frac{v_1+v_2x_i - y_i}{y_i} \right ) ^2
\tag{Exercise 8.17}
\]

Solution:
\[
\begin{pmatrix}
v_1  \\[0.3em]
v_2
\end{pmatrix}
=
\frac{1}{ad-b^2} \!
\begin{pmatrix}
a   \,\,&\,\, -b  \\[0.3em]
-b \,\,&\,\, d
\end{pmatrix}
 \!\!
\begin{pmatrix}
\sum 1/y_i  \\[0.3em]
\sum  x_i/y_i 
\end{pmatrix}
\]

\bigskip
\hspace{1in} where $a=\sum x_i^2/y_i^2$, $b=\sum x_i/y_i^2$, and $d=\sum 1/y_i^2$


\bigskip\bigskip\bigskip\noindent
\textbf{General} 

\bigskip\noindent
Error Function:
\[
E(\mathbf{v}) = ||\mathbf{A}\mathbf{v}-\mathbf{y}||_2^2
\tag{8.12}
\]

Moore-Penrose Solution:
\[
 \mathbf{v} =\mathbf{A}^+ \mathbf{y}
 \]

\hspace{1in} where 
\[
\mathbf{A}^+ \equiv  (\mathbf{A}^T\mathbf{A})^{-1} \mathbf{A}^T
\tag{8.25}
\]

\medskip
QR Solution (GS version):
\[
\mathbf{R}_m\mathbf{v} = \mathbf{y}_m 
\tag{8.22}
\]

\bigskip
\hspace{1in} where $\mathbf{R}_m=\mathbf{G}^T \mathbf{A}$, $\mathbf{y}_m=\mathbf{G}^T\mathbf{y}$, and $\mathbf{G}=\text{GS}(\mathbf{A})$

\bigskip\bigskip
SVD Solution: $\mathbf{A}=\mathbf{U}\mathbf{\Sigma}\mathbf{V}^T$
\[
\mathbf{A}^+= \mathbf{V}\mathbf{\Sigma}^{-T}\mathbf{U}^T
\tag{Exercise 8.7}
\]





 \end{document}
 

